UntypedAST.v
@@ -49,31 +49,9 @@ Inductive expr
 (* | IfThenElse (cond yes no: expr) *)
  | PrivateOrBuiltinCall (name: string) (args: list expr).
 
-(** Get the set of functions called by an expression. *)
-Fixpoint expr_callset (e: expr)
-: string_set
-:= let _ := string_set_impl in
-   match e with
-   | Const _ | LocalVar _ | StorageVar _ => empty
-   | UnOp _ a => expr_callset a
-   | BinOp _ a b => union (expr_callset a) (expr_callset b)
-(*   | IfThenElse a b c => union (expr_callset a) (union (expr_callset b) (expr_callset c)) *)
-   | PrivateOrBuiltinCall name args =>
-      let expr_list_callset := fix expr_list_callset (exprs: list expr) :=
-         match exprs with
-         | nil => empty
-         | (h :: t)%list => union (expr_callset h) (expr_list_callset t)
-         end
-      in add (expr_list_callset args) name
-   end.
-Fixpoint expr_list_callset (exprs: list expr)
-: string_set
-:= let _ := string_set_impl in
-   match exprs with
-   | nil => empty
-   | (h :: t)%list => union (expr_callset h) (expr_list_callset t)
-   end.
-
+(** "Small statement" is a term used in Python grammar, also in rust-vyper grammar.
+    Here we don't count local variable declarations as small statements.
+ *)
 Inductive small_stmt
 := Pass
  | Break
@@ -83,59 +61,17 @@ Inductive small_stmt
  | Raise (error: expr)
  | Assert (cond: expr) (error: option expr)
 (* | Log *)
- | LocalVarDecl (name: string) (init: option expr)
  | Assign (lhs: assignable) (rhs: expr)
  | BinOpAssign (lhs: assignable) (op: binop) (rhs: expr)
  | ExprStmt (e: expr).
 
-Definition small_stmt_callset (s: small_stmt)
-:= let _ := string_set_impl in
-   match s with
-   | Pass | Break | Continue | Return None | Revert | LocalVarDecl _ None => empty
-   | Return (Some e) | LocalVarDecl _ (Some e) | Raise e | Assert e None | ExprStmt e =>
-       expr_callset e
-   | Assign lhs rhs | BinOpAssign lhs _ rhs => expr_callset rhs
-   | Assert cond (Some error) => union (expr_callset cond) (expr_callset error)
-   end.
 
 Inductive stmt
 := SmallStmt (s: small_stmt)
+ | LocalVarDecl (name: string) (init: option expr)
  | IfElseStmt (cond: expr) (yes: list stmt) (no: option (list stmt))
  | FixedRangeLoop (var: string) (start: option uint256) (stop: uint256) (body: list stmt)
  | FixedCountLoop (var: string) (start: string) (count: uint256) (body: list stmt).
-
-Fixpoint stmt_callset (s: stmt)
-:= let _ := string_set_impl in
-   let stmt_list_callset := fix stmt_list_callset (stmts: list stmt) :=
-         match stmts with
-         | nil => empty
-         | (h :: t)%list => union (stmt_callset h) (stmt_list_callset t)
-         end
-   in match s with
-   | SmallStmt a => small_stmt_callset a
-   | IfElseStmt cond yes None => union (expr_callset cond) (stmt_list_callset yes)
-   | IfElseStmt cond yes (Some no) => union (expr_callset cond)
-                                            (union (stmt_list_callset yes) (stmt_list_callset no))
-   | FixedRangeLoop var start _ body | FixedCountLoop var start _ body =>
-       stmt_list_callset body
-   end.
-
-Fixpoint stmt_list_callset (stmts: list stmt)
-:= let _ := string_set_impl in
-   match stmts with
-   | nil => empty
-   | (h :: t)%list => union (stmt_callset h) (stmt_list_callset t)
-   end.
-
-Definition stmt_list_callset' (stmts: list stmt)
-:= let _ := string_set_impl in fold_right union empty (map stmt_callset stmts).
-
-Lemma stmt_list_callset_alt (s: list stmt):
-  stmt_list_callset s = stmt_list_callset' s.
-Proof.
-induction s. { easy. }
-cbn. f_equal. apply IHs.
-Qed.
 
 Inductive decl
 := (* ImportDecl
@@ -143,18 +79,12 @@ Inductive decl
       InterfaceDecl
       StructDecl *)
   StorageVarDecl (name: string)
-| FunDecl (name: string) (args: list string) (body: list stmt).
+| FunDecl (name: string) (args: list string) (body: expr). (* body: list stmt *)
 
 Definition decl_name (d: decl)
 : string
 := match d with
    | StorageVarDecl name | FunDecl name _ _ => name
-   end.
-
-Definition decl_callset (d: decl)
-:= let _ := string_set_impl in match d with
-   | StorageVarDecl _ => empty
-   | FunDecl name args body => stmt_list_callset body
    end.
 
 End AST.
