Callset.v
@@ -1,0 +1,176 @@
+From Coq Require Import List String.
+Require Import FSet Config UntypedAST.
+
+Section Callset.
+
+Context {C: VyperConfig}.
+
+(** Get the set of functions called by an expression. *)
+Fixpoint expr_callset (e: expr)
+: string_set
+:= let _ := string_set_impl in
+   match e with
+   | Const _ | LocalVar _ | StorageVar _ => empty
+   | UnOp _ a => expr_callset a
+   | BinOp _ a b => union (expr_callset a) (expr_callset b)
+(*   | IfThenElse a b c => union (expr_callset a) (union (expr_callset b) (expr_callset c)) *)
+   | PrivateOrBuiltinCall name args =>
+      let expr_list_callset := fix expr_list_callset (exprs: list expr) :=
+         match exprs with
+         | nil => empty
+         | (h :: t)%list => union (expr_callset h) (expr_list_callset t)
+         end
+      in add (expr_list_callset args) name
+   end.
+Fixpoint expr_list_callset (exprs: list expr)
+: string_set
+:= let _ := string_set_impl in
+   match exprs with
+   | nil => empty
+   | (h :: t)%list => union (expr_callset h) (expr_list_callset t)
+   end.
+
+Definition small_stmt_callset (s: small_stmt)
+:= let _ := string_set_impl in
+   match s with
+   | Pass | Break | Continue | Return None | Revert => empty
+   | Return (Some e) | Raise e | Assert e None | ExprStmt e =>
+       expr_callset e
+   | Assign lhs rhs | BinOpAssign lhs _ rhs => expr_callset rhs
+   | Assert cond (Some error) => union (expr_callset cond) (expr_callset error)
+   end.
+
+Fixpoint stmt_callset (s: stmt)
+:= let _ := string_set_impl in
+   let stmt_list_callset := fix stmt_list_callset (stmts: list stmt) :=
+         match stmts with
+         | nil => empty
+         | (h :: t)%list => union (stmt_callset h) (stmt_list_callset t)
+         end
+   in match s with
+   | SmallStmt a => small_stmt_callset a
+   | LocalVarDecl _ None => empty
+   | LocalVarDecl _ (Some e) => expr_callset e
+   | IfElseStmt cond yes None => union (expr_callset cond) (stmt_list_callset yes)
+   | IfElseStmt cond yes (Some no) => union (expr_callset cond)
+                                            (union (stmt_list_callset yes) (stmt_list_callset no))
+   | FixedRangeLoop var start _ body | FixedCountLoop var start _ body =>
+       stmt_list_callset body
+   end.
+
+Fixpoint stmt_list_callset (stmts: list stmt)
+:= let _ := string_set_impl in
+   match stmts with
+   | nil => empty
+   | (h :: t)%list => union (stmt_callset h) (stmt_list_callset t)
+   end.
+
+Definition stmt_list_callset' (stmts: list stmt)
+:= let _ := string_set_impl in fold_right union empty (map stmt_callset stmts).
+
+Lemma stmt_list_callset_alt (s: list stmt):
+  stmt_list_callset s = stmt_list_callset' s.
+Proof.
+induction s. { easy. }
+cbn. f_equal. apply IHs.
+Qed.
+
+Definition decl_callset (d: decl)
+:= let _ := string_set_impl in match d with
+   | StorageVarDecl _ => empty
+   | FunDecl name args body => (* XXX stmt_list_callset *) expr_callset body
+   end.
+
+Lemma callset_descend_unop {e a: expr} {op: unop}
+                           {allowed_calls: string_set}
+                           (E: e = UnOp op a)
+                           (ok: let _ := string_set_impl in
+                                FSet.is_subset (expr_callset e) allowed_calls = true):
+  let _ := string_set_impl in
+  FSet.is_subset (expr_callset a) allowed_calls = true.
+Proof.
+subst e. apply ok.
+Qed.
+
+Lemma callset_descend_binop_left {e a b: expr} {op: binop}
+                                 {allowed_calls: string_set}
+                                 (E: e = BinOp op a b)
+                                 (ok: let _ := string_set_impl in
+                                      FSet.is_subset (expr_callset e) allowed_calls = true):
+  let _ := string_set_impl in
+  FSet.is_subset (expr_callset a) allowed_calls = true.
+Proof. 
+subst e. cbn in ok.
+apply (FSet.is_subset_trans (FSet.union_subset_l _ _) ok).
+Qed.
+
+Lemma callset_descend_binop_right {e a b: expr} {op: binop}
+                                  {allowed_calls: string_set}
+                                  (E: e = BinOp op a b)
+                                  (ok: let _ := string_set_impl in
+                                       FSet.is_subset (expr_callset e) allowed_calls = true):
+  let _ := string_set_impl in
+  FSet.is_subset (expr_callset b) allowed_calls = true.
+Proof. 
+subst e. cbn in ok.
+apply (FSet.is_subset_trans (FSet.union_subset_r _ _) ok).
+Qed.
+
+Lemma callset_leaf {e: expr} {name: string} {args: list expr}
+                   {allowed_calls: string_set}
+                   (E: e = PrivateOrBuiltinCall name args)
+                   (ok: let _ := string_set_impl in
+                         FSet.is_subset (expr_callset e) allowed_calls = true):
+  let _ := string_set_impl in
+  FSet.has allowed_calls name = true.
+Proof.
+subst e. cbn in ok.
+rewrite FSet.is_subset_ok in ok.
+assert (Ok := ok name). clear ok.
+rewrite FSet.add_ok in Ok.
+destruct (string_dec name name). 2:{ tauto. }
+cbn.
+destruct (FSet.has allowed_calls name). { trivial. }
+cbn in Ok. discriminate.
+Qed.
+
+Lemma callset_descend_args {e: expr} {name: string} {args: list expr}
+                           {allowed_calls: string_set}
+                           (E: e = PrivateOrBuiltinCall name args)
+                           (ok: let _ := string_set_impl in
+                                FSet.is_subset (expr_callset e) allowed_calls = true):
+  let _ := string_set_impl in
+  FSet.is_subset (expr_list_callset args) allowed_calls = true.
+Proof.
+subst e. cbn in *.
+unfold expr_list_callset.
+apply (FSet.is_subset_trans (FSet.add_subset _ _) ok).
+Qed.
+
+
+Lemma callset_descend_head {h: expr} {t e: list expr}
+                           {allowed_calls: string_set}
+                           (E: e = (h :: t)%list)
+                           (ok: let _ := string_set_impl in
+                           FSet.is_subset (expr_list_callset e) allowed_calls = true):
+  let _ := string_set_impl in
+  FSet.is_subset (expr_callset h) allowed_calls = true.
+Proof. 
+subst e. cbn in ok.
+apply (FSet.is_subset_trans (FSet.union_subset_l _ _) ok).
+Qed.
+
+Lemma callset_descend_tail {h: expr} {t e: list expr}
+                           {allowed_calls: string_set}
+                           (E: e = (h :: t)%list)
+                           (ok: let _ := string_set_impl in
+                           FSet.is_subset (expr_list_callset e) allowed_calls = true):
+  let _ := string_set_impl in
+  FSet.is_subset (expr_list_callset t) allowed_calls = true.
+Proof. 
+subst e. cbn in ok.
+apply (FSet.is_subset_trans (FSet.union_subset_r _ _) ok).
+Qed.
+
+
+End Callset.
