Graph/Cycle.v
@@ -1,0 +1,97 @@
+From Coq Require Import List.
+
+Require Path.
+
+Record cycle {V: Type} (R: V -> V -> Prop)
+:= { vertex: V;
+     path: Path.t R vertex;
+     Closed: Path.endpoint path = vertex;
+     Nonempty: Path.is_empty path = false;
+   }.
+Arguments vertex   {_ _}.
+Arguments path     {_ _}.
+Arguments Closed   {_ _}.
+Arguments Nonempty {_ _}.
+Definition t {V: Type} := @cycle V.
+
+Local Lemma from_return_helper {V: Type}
+                               {R: V -> V -> Prop}
+                               {start: V}
+                               {p: Path.t R start}
+                               {a b: list V}
+                               (Return: Path.vertices p = a ++ start :: b):
+  Path.is_empty (Path.firstn (S (length a)) p) = false.
+Proof.
+rewrite Path.is_empty_false.
+rewrite Path.firstn_vertices.
+destruct Path.vertices. 2:{ easy. }
+symmetry in Return.
+apply app_eq_nil in Return.
+now destruct Return.
+Qed.
+
+Local Definition from_return {V: Type}
+                             {R: V -> V -> Prop}
+                             {start: V}
+                             {p: Path.t R start}
+                             {a b: list V}
+                             (Return: Path.vertices p = a ++ start :: b)
+: cycle R
+:= {| vertex := start
+    ; path := Path.firstn (S (length a)) p
+    ; Closed := Path.firstn_endpoint p Return
+    ; Nonempty := from_return_helper Return
+    |}.
+
+
+Local Lemma from_dup_nil {V: Type}
+                         {R: V -> V -> Prop}
+                         {start: V}
+                         {p: Path.t R start}
+                         {v: V}
+                         {a b c: list V}
+                         (Dup: Path.vertices_with_start p = a ++ v :: b ++ v :: c)
+                         (E : a = nil):
+  Path.vertices p = b ++ start :: c.
+Proof.
+subst. unfold Path.vertices_with_start in Dup.
+rewrite app_nil_l in Dup.
+inversion Dup. subst start.
+assumption.
+Qed.
+
+Local Lemma from_dup_cons {V: Type}
+                          {R: V -> V -> Prop}
+                          {start: V}
+                          {p: Path.t R start}
+                          {v h: V}
+                          {a b c t: list V}
+                          (Dup: Path.vertices_with_start p = a ++ v :: b ++ v :: c)
+                          (E : a = h :: t):
+  Path.vertices_with_start (Path.rest p (Path.nonempty_if_has_two_vertices Dup)) 
+   =
+  t ++ v :: b ++ v :: c.
+Proof.
+unfold Path.vertices_with_start in *.
+subst a.
+destruct p; cbn in *.
+{
+  exfalso. inversion Dup. subst. symmetry in H1.
+  apply app_eq_nil in H1. destruct H1. discriminate.
+}
+inversion Dup. easy.
+Qed.
+
+(* Extract a cycle from a duplication in Path.vertices_with_start. *)
+Fixpoint from_dup {V: Type}
+                  {R: V -> V -> Prop}
+                  {start: V}
+                  {p: Path.t R start}
+                  {v: V}
+                  {a b c: list V}
+                  (Dup: Path.vertices_with_start p = a ++ v :: b ++ v :: c)
+: cycle R
+:= match a as a' return a = a' -> cycle R with
+   | nil => fun E => from_return (from_dup_nil Dup E)
+   | h :: t => fun E => from_dup (from_dup_cons Dup E)
+   end eq_refl.
