Interpret.v
@@ -1,0 +1,374 @@
+From Coq Require Import String Arith NArith.
+Require Import Config UntypedAST Callset.
+Require FSet Map.
+
+Local Open Scope list_scope.
+Local Open Scope string_scope.
+
+Inductive expr_result {C: VyperConfig} (result_type: Type)
+:= ExprSuccess (result: result_type)
+ | ExprError (msg: string).
+Arguments ExprSuccess {_ _}.
+Arguments ExprError {_ _}.
+
+Inductive stmt_abort (return_type: Type)
+:= AbortError (msg: string)
+ | AbortBreak
+ | AbortContinue
+ | AbortReturnFromFunction
+ | AbortReturnFromContract
+ | AbortRevert.
+
+Inductive stmt_result {C: VyperConfig} (return_type: Type)
+:= StmtSuccess
+ | StmtAbort (a: stmt_abort return_type).
+Arguments StmtSuccess {_ _}.
+Arguments StmtAbort {_ _}.
+
+(** XXX *)
+Definition interpret_unop {C: VyperConfig} (op: unop) (a: uint256)
+: expr_result uint256
+:= ExprSuccess a.
+
+(** XXX *)
+Definition interpret_binop {C: VyperConfig} (op: binop) (a b: uint256)
+: expr_result uint256
+:= ExprSuccess a.
+
+Record calldag {C: VyperConfig} := {
+  cd_declmap:  string -> option decl;
+  cd_depthmap: string -> option N;
+  cd_depthmap_ok:
+    forall name: string,
+      match cd_declmap name with
+      | None => True
+      | Some decl =>
+          match cd_depthmap name with
+          | None => False
+          | Some x =>
+              let _ := string_set_impl in
+              FSet.for_all (decl_callset decl)
+                           (fun callee => match cd_depthmap callee with
+                                          | None => false
+                                          | Some y => (y <? x)%N
+                                          end)
+               = true
+            end
+      end;
+}.
+
+Fixpoint bind_args {C: VyperConfig} (names: list string) (values: list uint256)
+: string + string_map uint256
+:= let _ := string_map_impl in
+   match names with
+   | nil => match values with
+            | nil => inr Map.empty
+            | _ => inl "function called with too many arguments"
+            end
+   | hn :: tn => match values with
+                 | nil => inl "function called with too few arguments"
+                 | hv :: tv =>
+                     match bind_args tn tv with
+                     | inl err => inl err
+                     | inr bindings =>
+                        match Map.lookup bindings hn with
+                        | Some _ => inl "error: duplicate variable name"
+                        | None => inr (Map.insert bindings hn hv)
+                        end
+                     end
+                 end
+   end.
+
+Local Lemma interpret_call_helper {C: VyperConfig}
+                                  {this_decl: decl}
+                                  {fun_name: string}
+                                  {arg_names: list string}
+                                  {body: expr}
+                                  (E: this_decl = FunDecl fun_name arg_names body):
+  let H := string_set_impl in FSet.is_subset (expr_callset body) (decl_callset this_decl) = true.
+Proof.
+subst this_decl. unfold decl_callset. apply FSet.is_subset_refl.
+Qed.
+
+Lemma call_descend {C: VyperConfig}
+                   {call_depth_bound new_call_depth_bound current_fun_depth: nat}
+                   (DepthOk : current_fun_depth < call_depth_bound)
+                   (cd : calldag)
+                   (this_fun_name: string)
+                   (this_decl: decl)
+                   (this_decl_ok: cd_declmap cd this_fun_name = Some this_decl)
+                   (current_fun_depth_ok:
+                     cd_depthmap cd this_fun_name = Some (N.of_nat current_fun_depth))
+                   (e : expr)
+                   (CallOk : let _ := string_set_impl in
+                             FSet.is_subset (expr_callset e) (decl_callset this_decl) = true)
+                   (Ebound : call_depth_bound = S new_call_depth_bound)
+                   (name : string)
+                   (args : list expr)
+                   (E : e = PrivateOrBuiltinCall name args):
+  match cd_depthmap cd name with
+    | Some y => (y <? N.of_nat new_call_depth_bound)%N
+    | None => false
+    end = true.
+Proof.
+subst e. cbn in CallOk.
+assert(HasName: let _ := string_set_impl in FSet.has (decl_callset this_decl) name = true).
+{
+  cbn.
+  apply (FSet.is_subset_if CallOk name).
+  apply FSet.add_has.
+}
+clear CallOk. cbn in HasName.
+assert (K := cd_depthmap_ok cd this_fun_name).
+rewrite this_decl_ok in K.
+rewrite current_fun_depth_ok in K.
+cbn in K.
+rewrite FSet.for_all_ok in K.
+assert (L := K name HasName). clear K.
+subst call_depth_bound.
+apply lt_n_Sm_le in DepthOk.
+destruct (cd_depthmap cd name). 2:{ assumption. }
+rewrite N.ltb_lt. rewrite N.ltb_lt in L.
+refine (N.lt_le_trans _ _ _ L _).
+rewrite<- N.compare_le_iff.
+rewrite<- Nat2N.inj_compare.
+rewrite Nat.compare_le_iff.
+exact DepthOk.
+Qed.
+
+Fixpoint interpret_call {C: VyperConfig}
+                        (CALL_depth_bound: nat)
+                        (call_depth_bound: nat)
+                        (current_fun_depth: nat)
+                        (DepthOk: current_fun_depth < call_depth_bound)
+                        (cd: calldag)
+                        (world: world_state)
+                        (fun_name: string)
+                        (arg_values: list uint256)
+: world_state * expr_result uint256
+:= match cd_declmap cd fun_name with
+   | Some this_decl =>
+      match this_decl as this_decl' return this_decl = this_decl' -> _ with
+      | FunDecl _ arg_names body => fun E =>
+          match bind_args arg_names arg_values with
+          | inl err => (world, ExprError err)
+          | inr loc => interpret_expr CALL_depth_bound call_depth_bound
+                                      current_fun_depth DepthOk
+                                      cd this_decl
+                                      world loc body
+                                      (interpret_call_helper E)
+          end
+     | _ => fun _ => (world, ExprError "a declaration is found but it's not a function")
+     end eq_refl
+   | None => (world, ExprError "declaration not found") (* XXX: builtins *)
+   end
+with interpret_expr {C: VyperConfig}
+                    (CALL_depth_bound: nat)
+                    (call_depth_bound: nat)
+                    (current_fun_depth: nat)
+                    (DepthOk: current_fun_depth < call_depth_bound)
+                    (cd: calldag)
+                    (this_decl: decl)
+                    (world: world_state)
+                    (loc: string_map uint256)
+                    (e: expr)
+                    (CallOk: let _ := string_set_impl in 
+                             FSet.is_subset (expr_callset e) (decl_callset this_decl) = true)
+: world_state * expr_result uint256
+:= let interpret_expr_list := 
+     fix interpret_expr_list {C: VyperConfig}
+                             (CALL_depth_bound: nat)
+                             (call_depth_bound: nat)
+                             (current_fun_depth: nat)
+                             (DepthOk: current_fun_depth < call_depth_bound)
+                             (cd: calldag)
+                             (this_decl: decl)
+                             (world: world_state)
+                             (loc: string_map uint256)
+                             (e: list expr)
+                             (CallOk: let _ := string_set_impl in 
+                                      FSet.is_subset (expr_list_callset e) (decl_callset this_decl) = true)
+     {struct e}
+     : world_state * expr_result (list uint256)
+     := match e as e' return e = e' -> _ with
+        | nil => fun _ => (world, ExprSuccess nil)
+        | (h :: t)%list => fun E =>
+            let (world', result_h) := interpret_expr CALL_depth_bound call_depth_bound
+                                                     current_fun_depth DepthOk
+                                                     cd this_decl
+                                                     world loc h
+                                                     (callset_descend_head E CallOk)
+            in match result_h with
+               | ExprError msg => (world', ExprError msg)
+               | ExprSuccess x =>
+                  let (world'', result_t) := interpret_expr_list CALL_depth_bound call_depth_bound
+                                                                 current_fun_depth DepthOk
+                                                                 cd this_decl
+                                                                 world' loc t
+                                                                 (callset_descend_tail E CallOk)
+                  in (world'', match result_t with
+                               | ExprError _ => result_t
+                               | ExprSuccess y => ExprSuccess (x :: y)%list
+                               end)
+                end
+        end eq_refl
+   in match CALL_depth_bound as CALL_depth_bound' return CALL_depth_bound = CALL_depth_bound' -> _
+   with
+   | O => fun _ => (world, ExprError "Max CALL stack depth exceeded")
+   | S new_CALL_depth_bound => fun _ =>
+        match call_depth_bound as call_depth_bound'
+          return call_depth_bound = call_depth_bound' -> _
+        with
+        | O => fun E => False_rect _ (Nat.nlt_0_r current_fun_depth
+                                                  (eq_ind _ _ DepthOk _ E))
+        | S new_call_depth_bound => fun _ =>
+
+            match e as e' return e = e' -> _ with
+               | Const val => fun _ => (world, ExprSuccess val)
+               | LocalVar name => fun _ =>
+                   let _ := string_map_impl in
+                   (world, match Map.lookup loc name with
+                           | Some val => ExprSuccess val
+                           | None => ExprError "Local variable not found"
+                           end)
+               | StorageVar name => fun _ => 
+                   let _ := string_map_impl in
+                   (world, match storage_lookup world name with
+                           | Some val => ExprSuccess val
+                           | None => ExprError "Storage variable not found"
+                           end)
+               | UnOp op a => fun E =>
+                   let (world', result) := interpret_expr CALL_depth_bound call_depth_bound
+                                                          current_fun_depth DepthOk cd
+                                                          this_decl world loc a
+                                                          (callset_descend_unop E CallOk)
+                   in (world', match result with
+                               | ExprSuccess val => interpret_unop op val
+                               | ExprError msg => result
+                               end)
+               | BinOp op a b => fun E =>
+                   let (world', result_a) := interpret_expr CALL_depth_bound call_depth_bound
+                                                            current_fun_depth DepthOk cd
+                                                            this_decl world loc a
+                                                            (callset_descend_binop_left E CallOk)
+                   in match result_a with
+                   | ExprError msg => (world', result_a)
+                   | ExprSuccess x =>
+                     let (world'', result_b) := interpret_expr CALL_depth_bound call_depth_bound
+                                                               current_fun_depth DepthOk cd
+                                                               this_decl world' loc b
+                                                               (callset_descend_binop_right E CallOk)
+                     in (world'', match result_b with
+                                  | ExprError msg => result_b
+                                  | ExprSuccess y => interpret_binop op x y
+                                  end)
+                   end
+               (* | IfThenElse cond yes no => fun E =>
+                   _ *)
+               | PrivateOrBuiltinCall name args => fun E =>
+                   let (world', result_args) :=
+                     interpret_expr_list CALL_depth_bound call_depth_bound
+                                         current_fun_depth DepthOk cd
+                                         this_decl world loc args
+                                         (callset_descend_args E CallOk)
+                   in match result_args with
+                      | ExprError msg => (world', ExprError msg)
+                      | ExprSuccess arg_values =>
+                          _
+(*
+                          interpret_call CALL_depth_bound new_call_depth_bound
+                                         XXX
+                        (current_fun_depth: nat)
+                        (DepthOk: current_fun_depth < call_depth_bound)
+                        (cd: calldag)
+                        (world: world_state)
+                        (fun_name: string)
+                        (arg_values: list uint256) *)
+                      end
+               end eq_refl
+        end eq_refl
+   end eq_refl.
+
+
+Definition interpret_expr {C: VyperConfig}
+                          (CALL_depth_bound: nat)
+                          (call_depth_bound: nat)
+                          (current_fun_depth: nat)
+                          (DepthOk: current_fun_depth < call_depth_bound)
+                          (cd: calldag)
+                          (allowed_calls: string_set)
+                          (world: world_state)
+                          (loc: string_map uint256)
+                          (e: expr)
+                          (CallOk: let _ := string_set_impl in 
+                                   FSet.is_subset (expr_callset e) allowed_calls = true)
+: world_state * expr_result uint256. admit. Admitted.
+
+Definition stmt_is_local_var_decl {C: VyperConfig} (s: stmt)
+:= match s with
+   | LocalVarDecl _ _ => true
+   | _ => false
+   end.
+
+Fixpoint interpret_call {C: VyperConfig}
+                        (call_depth_bound: nat)
+                        (cd: calldag)
+                        (fun_name: string)
+                        (allowed_calls: string_set)
+                        (world: world_state)
+
+
+Fixpoint interpret_stmt {C: VyperConfig}
+                        (CALL_depth_bound: nat)
+                        (call_depth_bound: nat)
+                        (current_fun_depth: nat)
+                        (DepthOk: current_fun_depth < call_depth_bound)
+                        (cd: calldag)
+                        (allowed_calls: string_set)
+                        (world: world_state)
+                        (loc: string_map uint256)
+                        (return_type: Type)
+                        (s: stmt)
+                        (NotVarDecl: stmt_is_local_var_decl s = false)
+                        (CallOk: let _ := string_set_impl in 
+                                 FSet.is_subset (stmt_callset s) allowed_calls = true)
+: world_state * string_map uint256 * stmt_result return_type
+:= let interpret_loop := fix interpret_loop 
+   match s as s' return s = s' -> _ with
+   | SmallStmt ss => interpret_small_stmt XXXX
+   | LocalVarDecl _ _ => False_rect _ _
+   | IfElseStmt cond yes no =>
+      let (world', result_cond) := interpret_expr XXXXX
+   | FixedRangeLoop var start stop body =>
+      (* Range checks *)
+   | FixedCountLoop var start count body =>
+      (* Range checks *)
+   end eq_refl.
+Fixpoint interpret_stmt_list {C: VyperConfig}
+                             (CALL_depth_bound: nat)
+                             (call_depth_bound: nat)
+                             (current_fun_depth: nat)
+                             (DepthOk: current_fun_depth < call_depth_bound)
+                             (cd: calldag)
+                             (allowed_calls: string_set)
+                             (world: world_state)
+                             (loc: string_map uint256)
+                             (return_type: Type)
+                             (s: list stmt)
+                             (CallOk: let _ := string_set_impl in 
+                                      FSet.is_subset (stmt_list_callset s) allowed_calls = true)
+: world_state * string_map uint256 * stmt_result return_type
+:= match s with
+   | nil => (world, loc, StmtSuccess)
+   | LocalVarDecl name maybe_init :: rest =>
+      match Map.lookup loc name with
+      | Some _ => (world, StmtAbort (ErrorAbort "local variable shadowing"))
+      | None => _
+      end
+   | IfElseStmt cond yes no =>
+      
+   | FixedRangeLoop (var: string) (start: option uint256) (stop: uint256) (body: list stmt)
+   | FixedCountLoop (var: string) (start: string) (count: uint256) (body: list stmt).
+   end.
+
+Definition interpret 
